finished lock

ironfleet/src/Dafny/Distributed/Services/Lock/ShenghaoMain.i.dfy
@@ -23,7 +23,53 @@ module Main_i refines Main_s{
     import opened Refinement_i
     import opened MarshallProof_i
 
+    //=====================================DS_State=====================================
+
+    lemma OnlyMarshallableData(db:seq<DS_State>, config:Config)
+        requires |db| > 0;
+        requires DS_Init(db[0], config);
+        requires forall i {:trigger DS_Next(db[i], db[i+1])} :: 0 <= i < |db| - 1 ==> DS_Next(db[i], db[i+1]);
+        ensures forall i :: 0 <= i < |db| 
+                    ==> 
+                        forall p :: p in db[i].environment.sentPackets && p.src in db[i].servers
+                            ==> Demarshallable(p.msg, CMessageGrammar());
+    {
+        if (|db| == 1) {
+            assert(|db[0].environment.sentPackets| == 0);
+        }
+        else {
+            OnlyMarshallableData(db[0..|db| - 1], config);
+            var i := |db| - 2;
+            assert(DS_Next(db[i], db[i + 1]));
+            
+            if db[i].environment.nextStep.LEnvStepHostIos? && db[i].environment.nextStep.actor in db[i].servers {
+                assert(DS_NextOneServer(db[i], db[i + 1], db[i].environment.nextStep.actor, db[i].environment.nextStep.ios));
+                assert(OnlySentMarshallableData(db[i].environment.nextStep.ios));
+                var ios := db[i].environment.nextStep.ios;
+                var e := db[i].environment;
+                var e' := db[i + 1].environment;
+                if (e.nextStep.LEnvStepHostIos?) {
+                    assert(forall p :: p in e.sentPackets && p.src in db[i].servers ==> Demarshallable(p.msg, CMessageGrammar()));
+                    assert(e'.sentPackets == e.sentPackets + (set io | io in ios && io.LIoOpSend? :: io.s));
+                    assert(forall p :: p in ios && p.LIoOpSend? ==>  Demarshallable(p.s.msg, CMessageGrammar()));
+                    assert(forall p :: p in e'.sentPackets && p.src in db[i].servers ==> Demarshallable(p.msg, CMessageGrammar()));
+                }
+                else {
+                    assert(e'.sentPackets == e.sentPackets);
+                }
+            }
+            else {
+                assert(forall p :: p in db[i + 1].environment.sentPackets && p.src in db[i + 1].servers ==> p in db[i].environment.sentPackets);
+            }
+        }
+    }
+
+    //=====================================LS_State=====================================
+
     function AbstractifyConcretePacket(p:LPacket<EndPoint,seq<byte>>) : LPacket<EndPoint, LockMessage>
+        ensures p.dst == AbstractifyConcretePacket(p).dst;
+        ensures p.src == AbstractifyConcretePacket(p).src;
+        ensures AbstractifyCMessage(DemarshallData(p.msg)) == AbstractifyConcretePacket(p).msg;
     {
         LPacket(p.dst, p.src, AbstractifyCMessage(DemarshallData(p.msg)))
     }
@@ -34,6 +80,7 @@ module Main_i refines Main_s{
     }
 
     function LockSentPackets(m: set<LPacket<EndPoint, seq<byte>>>): set<LPacket<EndPoint, LockMessage>>
+        ensures forall msg :: msg in m ==> AbstractifyConcretePacket(msg) in LockSentPackets(m);
     {
         set k | k in m:: AbstractifyConcretePacket(k)
     }
@@ -221,10 +268,99 @@ module Main_i refines Main_s{
 
     function DSStateToLSState(ds:DS_State, config:ConcreteConfiguration): LS_State
         reads *;
-        ensures mapdomain(ds.servers) == mapdomain(DSStateToLSState(ds, config).servers);
+        ensures mapdomain(ds.servers) == mapdomain(DSStateToLSState(ds, config).servers); 
     {
         LS_State(LEnvToLockEnv(ds.environment), HostStateMapToNodeMap(ds.servers, config))
     }
+
+    lemma DStoLS(config:ConcreteConfiguration, db:seq<DS_State>) returns (lb:seq<LS_State>)
+        requires |db| > 0;
+        requires DS_Init(db[0], config);
+        requires forall i {:trigger DS_Next(db[i], db[i+1])} :: 0 <= i < |db| - 1 ==> DS_Next(db[i], db[i+1]);
+        ensures |db| == |lb|;
+        ensures LS_Init(lb[0], config);
+        ensures forall i :: 0 <= i < |lb| ==> forall m :: m in lb[i].servers <==> m in db[i].servers;
+        ensures lb[|lb| - 1] == DSStateToLSState(db[|db| - 1], config);
+        ensures forall i :: 0 <= i < |db| ==> forall m :: m in db[i].environment.sentPackets ==> AbstractifyConcretePacket(m) in lb[i].environment.sentPackets;
+        ensures forall i{:trigger LS_Next(lb[i], lb[i + 1])} :: 0 <= i < |lb| - 1 ==> LS_Next(lb[i], lb[i + 1]);
+    {
+        if (|db| == 1) {
+            assert(ValidConfig(config));
+            assert(SeqIsUnique(config));
+            assert(|config| > 0);
+            assert(ConcreteConfigInit(config, mapdomain(db[0].servers), db[0].clients));
+            assert(forall e :: e in config <==> e in db[0].servers);
+            assert(LEnvironment_Init(db[0].environment));
+            lb := [DSStateToLSState_Init(db[0], config)];
+        }
+        else {
+            var prev := DStoLS(config, db[0..|db| - 1]);
+            var k := |db| - 2;
+            var s := DSStateToLSState(db[k], config);
+            var s' := DSStateToLSState(db[k + 1], config);
+            assert(prev[|prev| - 1] == s);
+            lb := prev + [s'];
+            assert(0 <= k < |db| - 1);
+            assert(DS_Next(db[k], db[k + 1]));
+            assert(IsValidLEnvStep(db[|db| - 2].environment, db[|db| - 2].environment.nextStep));
+            assert(s.environment == LEnvToLockEnv(db[|db| - 2].environment));
+            LEnvironmentToLockEnvValidNextStep(db[|db| - 2].environment);
+            assert(LEnvironment_Next(s.environment,
+                                     s'.environment));
+            if (s.environment.nextStep.LEnvStepHostIos? && s.environment.nextStep.actor in s.servers) {
+                assert(NodeNext(s.servers[s.environment.nextStep.actor], s'.servers[s.environment.nextStep.actor], s.environment.nextStep.ios));
+            }
+            else {
+                assert(s'.servers == s.servers);
+            }
+            assert(LS_Next(s, s'));
+        }
+    }
+
+    //=====================================GLS_State=====================================
+
+    function LSStateToGLSState(ls:LS_State, gls_prev:GLS_State, config:ConcreteConfiguration) : GLS_State
+        requires LS_Next(gls_prev.ls, ls);
+        ensures GLS_Next(gls_prev, LSStateToGLSState(ls, gls_prev, config));
+    {
+        if gls_prev.ls.environment.nextStep.LEnvStepHostIos? && gls_prev.ls.environment.nextStep.actor in gls_prev.ls.servers
+            && NodeGrant(gls_prev.ls.servers[gls_prev.ls.environment.nextStep.actor], ls.servers[gls_prev.ls.environment.nextStep.actor], gls_prev.ls.environment.nextStep.ios)
+            && gls_prev.ls.servers[gls_prev.ls.environment.nextStep.actor].held && gls_prev.ls.servers[gls_prev.ls.environment.nextStep.actor].epoch < 0xFFFF_FFFF_FFFF_FFFF then
+            GLS_State(ls, gls_prev.history + [gls_prev.ls.servers[gls_prev.ls.environment.nextStep.actor].config[(gls_prev.ls.servers[gls_prev.ls.environment.nextStep.actor].my_index + 1) % |gls_prev.ls.servers[gls_prev.ls.environment.nextStep.actor].config|]])
+        else GLS_State(ls, gls_prev.history)
+    }
+
+    lemma LSToGLS(lb:seq<LS_State>, config:ConcreteConfiguration) returns (glb:seq<GLS_State>) 
+        requires |lb| > 0;
+        requires LS_Init(lb[0], config);
+        requires forall i{:trigger LS_Next(lb[i], lb[i + 1])} :: 0 <= i < |lb| - 1 ==> LS_Next(lb[i], lb[i + 1]);
+        ensures |lb| == |glb|;
+        ensures GLS_Init(glb[0], config);
+        ensures forall i :: 0 <= i < |glb| ==> glb[i].ls == lb[i];
+        ensures forall i{:trigger GLS_Next(glb[i], glb[i + 1])} :: 0 <= i < |glb| - 1 ==> GLS_Next(glb[i], glb[i + 1])
+    {
+        if (|lb| == 1) {
+            var gls := GLS_State(lb[0], [config[0]]);
+            assert(GLS_Init(gls, config));
+            glb := [gls];
+        }
+        else {
+            var prev := LSToGLS(lb[0..|lb| - 1], config);
+            var gls_prev := prev[|prev| - 1];
+            var k := |lb| - 2;
+            assert(gls_prev.ls == lb[k]);
+            assert(LS_Next(lb[k], lb[k + 1]));
+            var gls_new := LSStateToGLSState(lb[k + 1], gls_prev, config);
+            assert(GLS_Next(gls_prev, gls_new));
+            var s := gls_prev.ls;
+            var s' := gls_new.ls;
+            assert(LS_Next(s, s'));
+            LS_ServerInvariant(s, s');
+            glb := prev + [gls_new];
+        }
+    }
+
+    //=========================================Invariant Proof===========================
 
     lemma LS_ServerInvariant(s:LS_State, s':LS_State)
         requires LS_Next(s, s');
@@ -268,89 +404,6 @@ module Main_i refines Main_s{
         }
     }
 
-    lemma DStoLS(config:ConcreteConfiguration, db:seq<DS_State>) returns (lb:seq<LS_State>)
-        requires |db| > 0;
-        requires DS_Init(db[0], config);
-        requires forall i {:trigger DS_Next(db[i], db[i+1])} :: 0 <= i < |db| - 1 ==> DS_Next(db[i], db[i+1]);
-        ensures |db| == |lb|;
-        ensures LS_Init(lb[0], config);
-        ensures lb[|lb| - 1] == DSStateToLSState(db[|db| - 1], config);
-        ensures forall i{:trigger LS_Next(lb[i], lb[i + 1])} :: 0 <= i < |lb| - 1 ==> LS_Next(lb[i], lb[i + 1]);
-        // ensures forall i{:trigger LS_Next(lb[i], lb[i + 1])} :: 0 <= i < |lb| - 1 ==> Collections__Maps2_s.mapdomain(lb[i].servers) == Collections__Maps2_s.mapdomain(lb[i + 1].servers);
-    {
-        if (|db| == 1) {
-            assert(ValidConfig(config));
-            assert(SeqIsUnique(config));
-            assert(|config| > 0);
-            assert(ConcreteConfigInit(config, mapdomain(db[0].servers), db[0].clients));
-            assert(forall e :: e in config <==> e in db[0].servers);
-            assert(LEnvironment_Init(db[0].environment));
-            lb := [DSStateToLSState_Init(db[0], config)];
-        }
-        else {
-            var prev := DStoLS(config, db[0..|db| - 1]);
-            var k := |db| - 2;
-            var s := DSStateToLSState(db[k], config);
-            var s' := DSStateToLSState(db[k + 1], config);
-            assert(prev[|prev| - 1] == s);
-            lb := prev + [s'];
-            assert(0 <= k < |db| - 1);
-            assert(DS_Next(db[k], db[k + 1]));
-            assert(IsValidLEnvStep(db[|db| - 2].environment, db[|db| - 2].environment.nextStep));
-            assert(s.environment == LEnvToLockEnv(db[|db| - 2].environment));
-            LEnvironmentToLockEnvValidNextStep(db[|db| - 2].environment);
-            assert(LEnvironment_Next(s.environment,
-                                     s'.environment));
-            if (s.environment.nextStep.LEnvStepHostIos? && s.environment.nextStep.actor in s.servers) {
-                assert(NodeNext(s.servers[s.environment.nextStep.actor], s'.servers[s.environment.nextStep.actor], s.environment.nextStep.ios));
-            }
-            else {
-                assert(s'.servers == s.servers);
-            }
-            assert(LS_Next(s, s'));
-        }
-    }
-
-    function LSStateToGLSState(ls:LS_State, gls_prev:GLS_State, config:ConcreteConfiguration) : GLS_State
-        requires LS_Next(gls_prev.ls, ls);
-        ensures GLS_Next(gls_prev, LSStateToGLSState(ls, gls_prev, config));
-    {
-        if gls_prev.ls.environment.nextStep.LEnvStepHostIos? && gls_prev.ls.environment.nextStep.actor in gls_prev.ls.servers
-            && NodeGrant(gls_prev.ls.servers[gls_prev.ls.environment.nextStep.actor], ls.servers[gls_prev.ls.environment.nextStep.actor], gls_prev.ls.environment.nextStep.ios)
-            && gls_prev.ls.servers[gls_prev.ls.environment.nextStep.actor].held && gls_prev.ls.servers[gls_prev.ls.environment.nextStep.actor].epoch < 0xFFFF_FFFF_FFFF_FFFF then
-            GLS_State(ls, gls_prev.history + [gls_prev.ls.servers[gls_prev.ls.environment.nextStep.actor].config[(gls_prev.ls.servers[gls_prev.ls.environment.nextStep.actor].my_index + 1) % |gls_prev.ls.servers[gls_prev.ls.environment.nextStep.actor].config|]])
-        else GLS_State(ls, gls_prev.history)
-    }
-
-    lemma LSToGLS(lb:seq<LS_State>, config:ConcreteConfiguration) returns (glb:seq<GLS_State>) 
-        requires |lb| > 0;
-        requires LS_Init(lb[0], config);
-        requires forall i{:trigger LS_Next(lb[i], lb[i + 1])} :: 0 <= i < |lb| - 1 ==> LS_Next(lb[i], lb[i + 1]);
-        ensures |lb| == |glb|;
-        ensures GLS_Init(glb[0], config);
-        ensures forall i :: 0 <= i < |glb| ==> glb[i].ls == lb[i];
-        ensures forall i{:trigger GLS_Next(glb[i], glb[i + 1])} :: 0 <= i < |glb| - 1 ==> GLS_Next(glb[i], glb[i + 1])
-    {
-        if (|lb| == 1) {
-            var gls := GLS_State(lb[0], [config[0]]);
-            assert(GLS_Init(gls, config));
-            glb := [gls];
-        }
-        else {
-            var prev := LSToGLS(lb[0..|lb| - 1], config);
-            var gls_prev := prev[|prev| - 1];
-            var k := |lb| - 2;
-            assert(gls_prev.ls == lb[k]);
-            assert(LS_Next(lb[k], lb[k + 1]));
-            var gls_new := LSStateToGLSState(lb[k + 1], gls_prev, config);
-            assert(GLS_Next(gls_prev, gls_new));
-            var s := gls_prev.ls;
-            var s' := gls_new.ls;
-            assert(LS_Next(s, s'));
-            LS_ServerInvariant(s, s');
-            glb := prev + [gls_new];
-        }
-    }
 
     lemma NodeNext_ConfigInvariant(s:Node, s':Node, ios:seq<LockIo>)
         requires NodeNext(s, s', ios);
@@ -435,71 +488,299 @@ module Main_i refines Main_s{
         }
     }
 
-    predicate GLSCor(s:GLS_State) {
-        forall p, epoch:: 
-            p in s.ls.environment.sentPackets 
-        && p.src in s.ls.servers 
-        && p.dst in s.ls.servers 
-        && p.msg == SBToLM(MarshallLockMsg(epoch))
-        ==>
-            1 <= epoch <= |s.history|
-        && p.src == s.history[epoch - 1]    
+    predicate LockInvariant(s:GLS_State, config:Config)
+    {
+        |s.history| >= 1 &&
+        (forall m :: m in s.history ==> m in s.ls.servers) &&
+        (forall ser :: ser in s.ls.servers && s.ls.servers[ser].held 
+                ==> 
+                    s.ls.servers[ser].epoch == |s.history|
+                    && ser == s.history[|s.history| - 1]) &&
+        (forall i :: 0 <= i < |s.history| - 1 
+                ==> 
+                    s.history[i] in s.ls.servers && s.ls.servers[s.history[i]].epoch >= i + 1) &&
+        (forall mt :: mt in s.ls.environment.sentPackets 
+                    && mt.src in s.ls.servers 
+                    && mt.msg.Transfer? 
+                ==> 
+                    0 <= mt.msg.transfer_epoch - 1 < |s.history|
+                    && s.history[mt.msg.transfer_epoch - 1] == mt.dst) &&
+        (forall ml :: ml in s.ls.environment.sentPackets
+                    && ml.src in s.ls.servers
+                    && ml.msg.Locked?
+                ==>
+                    1 <= ml.msg.locked_epoch <= |s.history|
+                    && s.history[ml.msg.locked_epoch - 1] == ml.src) &&
+        (forall mm :: mm in s.ls.servers <==> mm in config) &&
+        (forall ms :: ms in s.ls.servers ==> s.ls.servers[ms].config == config)
     }
 
-    lemma GLSHistoryGrowing(s:GLS_State, s':GLS_State)
+    lemma LockTransition(s: GLS_State, s':GLS_State, config:Config)
         requires GLS_Next(s, s');
-        requires GLSCor(s);
-        requires forall m :: m in s.ls.environment.sentPackets && m.msg.Transfer? ==> m.dst in s.history;
-        // ensures forall m :: m in s'.sentPackets && m.msg.Transfer? ==> m.dst in s'.history;
-        // ensures GLSCor(s');
+        requires LockInvariant(s, config);
+
+        ensures LockInvariant(s', config);
+        
     {
-        if (s.ls.environment.nextStep.LEnvStepHostIos? && s.ls.environment.nextStep.actor in s.ls.servers) {
-            var sa := s.ls.servers[s.ls.environment.nextStep.actor];
-            var sa' := s'.ls.servers[s.ls.environment.nextStep.actor];
-            var ios := s.ls.environment.nextStep.ios;
-            if (s.ls.environment.nextStep.LEnvStepHostIos? && s.ls.environment.nextStep.actor in s.ls.servers
-               && NodeGrant(s.ls.servers[s.ls.environment.nextStep.actor], s'.ls.servers[s.ls.environment.nextStep.actor], s.ls.environment.nextStep.ios)
-               && s.ls.servers[s.ls.environment.nextStep.actor].held && s.ls.servers[s.ls.environment.nextStep.actor].epoch < 0xFFFF_FFFF_FFFF_FFFF) {
-                var id := s.ls.environment.nextStep.actor;
-                
-            }
-            else if (NodeAccept(sa, sa', ios)) {
-                assert(s.history == s'.history);
-                assert(LS_Next(s.ls, s'.ls));
-                LS_ServerInvariant(s.ls, s'.ls);
-                if (!ios[0].LIoOpTimeoutReceive? 
-                    && !sa.held && ios[0].r.src in sa.config
-                    && ios[0].r.msg.Transfer? 
-                    && ios[0].r.msg.transfer_epoch > sa.epoch) {
-                    assert(s'.ls.environment.sentPackets == s.ls.environment.sentPackets + {ios[1].s});
-                    assert(ios[0].r in s.ls.environment.sentPackets);
-                    assert(ios[1].s.msg.locked_epoch == ios[0].r.msg.transfer_epoch);
-                    assert(forall epoch :: ios[1].s.msg == SBToLM(MarshallLockMsg(epoch)) ==> 1 <= epoch <= |s.history|);
+        var ls := s.ls;
+        var ls' := s'.ls;
+        assert(forall m :: m in ls.servers <==> m in ls'.servers);
+        assert(forall m :: m in s.ls.servers <==> m in config);
+        assert(forall m :: m in ls.servers ==> ls.servers[m].config == ls.servers[m].config);
+        assert(forall m :: m in ls'.servers <==> m in config);
+        if ls.environment.nextStep.LEnvStepHostIos? && ls.environment.nextStep.actor in ls.servers {
+            assert(LS_NextOneServer(ls, ls', ls.environment.nextStep.actor, ls.environment.nextStep.ios));
+            var ios := ls.environment.nextStep.ios;
+            var actor := ls.environment.nextStep.actor;
+            var node := ls.servers[actor];
+            var node' := ls'.servers[actor];
+            assert(ls'.servers == ls.servers[actor := ls'.servers[actor]]);
+            assert(actor in ls.servers);
+            assert(actor in ls'.servers);
+            if (NodeGrant(node, node', ios)) {
+                if node.held && node.epoch < 0xFFFF_FFFF_FFFF_FFFF {
+                    assert(s'.history == s.history + [node.config[(node.my_index + 1) % |node.config|]]);
+                    assert(node.config[(node.my_index + 1) % |node.config|] == ios[0].s.dst);
+                    assert(node.config[(node.my_index + 1) % |node.config|] in s'.ls.servers);
+                    assert(ios[0].s.msg.transfer_epoch == node.epoch + 1);
+                    assert(ios[0].s.msg.transfer_epoch == |s'.history|);
+                    assert(ls'.environment.sentPackets == ls.environment.sentPackets + {ios[0].s});
+                    assert(forall m :: m in s'.ls.environment.sentPackets 
+                                    && m.src in s'.ls.servers 
+                                    && m.msg.Transfer? 
+                                ==> 
+                                    0 <= m.msg.transfer_epoch - 1 < |s'.history|
+                                    && s'.history[m.msg.transfer_epoch - 1] == m.dst);
+                    assert(0 <= ios[0].s.msg.transfer_epoch - 1 < |s'.history|);
+                    assert(|s.history| >= 1);
+                    assert(|s'.history| >= 2);
+                    assert(node'.epoch == node.epoch == |s.history| == |s'.history| - 1);
+                    var i := |s'.history| - 2;
+                    assert(i == |s.history| - 1);
+                    assert(s'.history[i] == s.history[i] == actor);
+                    assert(s'.ls.servers[s'.history[i]].epoch == s.ls.servers[s.history[i]].epoch == i + 1);
+                    assert(forall ii :: 0 <= ii < |s'.history| - 1 
+                                ==> 
+                                  s'.history[ii] in s'.ls.servers && s'.ls.servers[s'.history[ii]].epoch >= ii + 1);
+                    assert(forall m :: m in ls.servers && ls.servers[m].held ==> m == s.history[i]);
+                    assert(forall m :: m in ls.servers && ls.servers[m].held ==> !ls'.servers[m].held);
+                    assert(forall m :: m in ls'.servers && ls'.servers[m].held ==> ls'.servers[m].epoch == |s'.history|);
+                    assert(
+                        forall m :: m in s'.ls.environment.sentPackets
+                                    && m.msg.Locked?
+                                ==>
+                                    m in s.ls.environment.sentPackets
+                    );
+                }
+                else  {
+                    assert(ls'.servers == ls.servers);
+                    assert(s'.history == s.history);
+                    assert(
+                        forall m :: m in ls'.environment.sentPackets 
+                                    && m.src in ls'.servers 
+                                    && m.msg.Transfer? 
+                        ==> m in ls.environment.sentPackets
+                    );
+                    assert(
+                        forall m :: m in s'.ls.environment.sentPackets
+                                && m.msg.Locked?
+                            ==>
+                                m in s.ls.environment.sentPackets
+                    );
                 }
             }
             else {
-                assert(s.history == s'.history);
-                assert(LS_Next(s.ls, s'.ls));
-                assert(s.ls.environment.sentPackets == s'.ls.environment.sentPackets);
-                LS_ServerInvariant(s.ls, s'.ls);
-                assert(GLSCor(s'));
+                assert(NodeAccept(node, node', ios));
+                if (ios[0].LIoOpTimeoutReceive?) {
+                    assert(ls'.servers == ls.servers);
+                    assert(s'.history == s.history);
+                    assert(
+                        forall m :: m in ls'.environment.sentPackets 
+                                    && m.src in ls'.servers 
+                                    && m.msg.Transfer? 
+                        ==> m in ls.environment.sentPackets
+                    );
+                    assert(
+                        forall m :: m in s'.ls.environment.sentPackets
+                                    && m.msg.Locked?
+                                ==>
+                                    m in s.ls.environment.sentPackets
+                    );
+                }
+                else if (!node.held 
+                         && ios[0].r.src in node.config
+                         && ios[0].r.msg.Transfer? 
+                         && ios[0].r.msg.transfer_epoch > node.epoch) {
+                    assert(s.history == s'.history);
+                    assert(ios[0].r in ls.environment.sentPackets && ios[0].r.src in ls.servers);
+                    assert(ios[0].r.dst in s.history);
+                    assert(IsValidLEnvStep(ls.environment, ls.environment.nextStep));
+                    assert(forall io :: io in ios ==> IsValidLIoOp(io, actor, ls.environment));
+                    assert(forall io :: io in ios && io.LIoOpReceive? ==> io.r.dst == actor);
+                    assert(ios[0].r.dst == actor);
+                    assert(exists i :: 0 <= i < |s.history| ==> s.history[i] == ios[0].r.dst);
+                    assert(forall i :: 0 <= i < |s.history| - 1 && s.history[i] == actor ==> node.epoch >= i + 1);
+                    assert(s.history[|s.history| - 1] == ios[0].r.dst);
+                    assert(node'.epoch > node.epoch);
+                    var m := ios[0].r;
+                    assert(forall i :: 0 <= i < |s.history| - 1 && s.history[i] == m.dst ==> m.msg.transfer_epoch > i + 1);
+                    assert(m.msg.transfer_epoch == |s.history|);
+                    assert(node'.held);
+                    assert(node'.epoch == m.msg.transfer_epoch == |s'.history|);
+                    assert(s'.history[|s'.history| - 1] == actor);
+                    assert(
+                        forall i :: 0 <= i < |s'.history| - 1 
+                            ==> 
+                                s'.history[i] in s'.ls.servers && s'.ls.servers[s'.history[i]].epoch >= i + 1
+                    );
+                    assert(ios[1].s.msg.locked_epoch == |s'.history|);
+                    assert(
+                        forall md :: md in s'.ls.environment.sentPackets
+                                    && md.msg.Locked?
+                                ==>
+                                    md in s.ls.environment.sentPackets
+                                    || md == ios[1].s
+                    );
+                }
+                else {
+                    assert(ls'.servers == ls.servers);
+                    assert(s'.history == s.history);
+                    assert(
+                        forall m :: m in ls'.environment.sentPackets 
+                                    && m.src in ls'.servers 
+                                    && m.msg.Transfer? 
+                        ==> m in ls.environment.sentPackets
+                    );
+                    assert(
+                        forall m :: m in s'.ls.environment.sentPackets
+                                    && m.msg.Locked?
+                                ==>
+                                    m in s.ls.environment.sentPackets
+                    );
+                }
             }
         }
-        else if (s.ls.environment.nextStep.LEnvStepHostIos? && !(s.ls.environment.nextStep.actor in s.ls.servers)) {
-            assert(s.history == s'.history);
-            assert(LS_Next(s.ls, s'.ls));
-            assert(forall m :: m in s'.ls.environment.sentPackets && m.src in s'.ls.servers ==> m in s.ls.environment.sentPackets);
-            LS_ServerInvariant(s.ls, s'.ls);
-            assert(GLSCor(s'));
-        }
         else {
-            assert(s.history == s'.history);
-            assert(s.ls.environment.sentPackets == s'.ls.environment.sentPackets);
-            assert(LS_Next(s.ls, s'.ls));
-            LS_ServerInvariant(s.ls, s'.ls);
-            assert(GLSCor(s'));
+            assert(ls'.servers == ls.servers);
+            assert(s'.history == s.history);
+            assert(
+                forall m :: m in ls'.environment.sentPackets 
+                            && m.src in ls'.servers 
+                            && m.msg.Transfer? 
+                ==> m in ls.environment.sentPackets
+            );
+            assert(
+                forall m :: m in s'.ls.environment.sentPackets
+                            && m.msg.Locked?
+                            && m.src in ls'.servers
+                        ==>
+                            m in s.ls.environment.sentPackets
+            );
         }
     }
+
+
+    lemma LockIsUnique(glb:seq<GLS_State>, config:Config) 
+        requires |glb| > 0;
+        requires GLS_Init(glb[0], config);
+        requires forall i{:trigger GLS_Next(glb[i], glb[i + 1])} :: 0 <= i < |glb| - 1 ==> GLS_Next(glb[i], glb[i + 1]);
+        ensures forall i :: 0 <= i < |glb| ==> LockInvariant(glb[i], config);
+    {
+        if (|glb| == 1) {
+            assert(GLS_Init(glb[0], config));
+            var servers := glb[0].ls.servers;
+            assert(forall index :: 0 <= index < |config| ==> NodeInit(servers[config[index]], index, config));
+            assert(forall m :: m in servers <==> m in config);
+            assert(forall m :: m in servers ==> servers[m].config == config);
+            assert(|glb[0].history| == 1);
+            assert(glb[0].history[0] in config);
+            assert(glb[0].history[0] in servers);
+            assert(forall m :: m in glb[0].history ==> m in servers);
+            assert(forall e :: e in config <==> e in servers);
+            assert(forall i :: 0 <= i < |config| ==> servers[config[i]].held == (i == 0));
+            assert(forall m :: m in servers && servers[m].held ==> m == config[0]);
+            assert(LockInvariant(glb[0], config));
+        } 
+        else {
+            LockIsUnique(glb[0..|glb| - 1], config);
+            var i := |glb| - 2;
+            assert(i >= 0);
+            assert(GLS_Next(glb[i], glb[i + 1]));
+            LockTransition(glb[i], glb[i + 1], config);
+            assert(LockInvariant(glb[|glb| - 1], config));
+        }
+    }
+
+    // =================================GLS Correspondence=========================================
+
+    predicate GLS_Correspondence(concretePkts:set<LPacket<EndPoint, seq<byte>>>, gls:GLS_State) 
+    {
+        forall p, epoch :: 
+            p in concretePkts 
+        && p.src in gls.ls.servers 
+        && p.dst in gls.ls.servers 
+        && p.msg == MarshallLockMsg(epoch) 
+        ==>
+            1 <= epoch <= |gls.history|
+        && p.src == gls.history[epoch-1]               
+    } 
+
+    lemma GLS_Correspondence_Proof(gls:GLS_State, config:Config, concretePkts:set<LPacket<EndPoint, seq<byte>>>)
+        requires LockInvariant(gls, config);
+        requires forall p :: p in concretePkts && p.src in gls.ls.servers 
+                        ==> 
+                            Demarshallable(p.msg, CMessageGrammar())
+                            && AbstractifyConcretePacket(p) in gls.ls.environment.sentPackets;
+        ensures GLS_Correspondence(concretePkts, gls);
+    {
+        forall p, epoch |
+                p in concretePkts 
+                && p.src in gls.ls.servers 
+                && p.dst in gls.ls.servers 
+                && p.msg == MarshallLockMsg(epoch) 
+            ensures 1 <= epoch <= |gls.history|;
+            ensures p.src == gls.history[epoch - 1];
+        {
+            var np := AbstractifyConcretePacket(p);
+            assert(Demarshallable(p.msg, CMessageGrammar()));
+            lemma_ParseMarshallLockedAbstract(p.msg, epoch, np.msg);
+            assert(np.msg.Locked?);
+            assert(np.msg.locked_epoch == epoch);
+            assert(np in gls.ls.environment.sentPackets);
+            assert(1 <= np.msg.locked_epoch <= |gls.history|);
+            assert(np.src == p.src);
+            assert(gls.history[np.msg.locked_epoch - 1] == np.src);
+        }
+    }
+
+    lemma GLS_Cor_Seq(db:seq<DS_State>, glb:seq<GLS_State>, config:Config)
+        requires |db| == |glb|;
+        requires forall i :: 0 <= i < |glb| ==> LockInvariant(glb[i], config);
+        requires forall i :: 0 <= i < |glb| ==> forall m :: m in glb[i].ls.servers <==> m in db[i].servers;
+        requires forall i :: 0 <= i < |db| 
+                        ==> 
+                            forall p :: p in db[i].environment.sentPackets && p.src in db[i].servers
+                                    ==> 
+                                        Demarshallable(p.msg, CMessageGrammar()) 
+                                        && AbstractifyConcretePacket(p) in glb[i].ls.environment.sentPackets;
+        ensures forall i :: 0 <= i < |glb| ==> GLS_Correspondence(db[i].environment.sentPackets, glb[i])
+    {
+        assert(
+            forall i :: 0 <= i < |db| 
+                ==> 
+                    forall p :: p in db[i].environment.sentPackets && p.src in glb[i].ls.servers
+                            ==> 
+                                Demarshallable(p.msg, CMessageGrammar()) 
+                                && AbstractifyConcretePacket(p) in glb[i].ls.environment.sentPackets
+        );
+        forall i | 0 <= i < |glb|
+            ensures GLS_Correspondence(db[i].environment.sentPackets, glb[i])
+        {
+            GLS_Correspondence_Proof(glb[i], config, db[i].environment.sentPackets);
+        }
+    }
+
+    //==========================================Service State=============================
 
     lemma GLSToSS(glb:seq<GLS_State>, config:ConcreteConfiguration) returns (sb:seq<ServiceState>)
         requires |glb| > 0;
@@ -570,8 +851,13 @@ module Main_i refines Main_s{
         // ensures  forall i {:trigger Service_Next(sb[i], sb[i+1])} :: 0 <= i < |sb| - 1 ==> sb[i] == sb[i+1] || Service_Next(sb[i], sb[i+1]);
         // ensures  forall i :: 0 <= i < |db| ==> Service_Correspondence(db[i].environment.sentPackets, sb[i]);
     {
+        OnlyMarshallableData(db, config);
         var lb := DStoLS(config, db);
         var glb := LSToGLS(lb, config);
+        assert(|glb| == |db|);
+        assert(forall i :: 0 <= i < |glb| ==> forall m :: m in db[i].environment.sentPackets ==> AbstractifyConcretePacket(m) in glb[i].ls.environment.sentPackets);
+        LockIsUnique(glb, config);
+        GLS_Cor_Seq(db, glb, config);
         sb := GLSToSS(glb, config);
     }
 }
